% Created 2020-04-08 Wed 19:09
% Intended LaTeX compiler: pdflatex
\documentclass[11pt]{article}
\usepackage[utf8]{inputenc}
\usepackage[T1]{fontenc}
\usepackage{graphicx}
\usepackage{grffile}
\usepackage{longtable}
\usepackage{wrapfig}
\usepackage{rotating}
\usepackage[normalem]{ulem}
\usepackage{amsmath}
\usepackage{textcomp}
\usepackage{amssymb}
\usepackage{capt-of}
\usepackage{hyperref}
\author{Dustin Leatherman}
\date{\today}
\title{Optimization Theory - Bonus Problem}
\hypersetup{
 pdfauthor={Dustin Leatherman},
 pdftitle={Optimization Theory - Bonus Problem},
 pdfkeywords={},
 pdfsubject={},
 pdfcreator={Emacs 26.3 (Org mode 9.4)}, 
 pdflang={English}}
\begin{document}

\maketitle
\tableofcontents


\section{Problem Statement}
\label{sec:org8628d76}

Let \(A \in R ^{m \times N}\), where \(m \leq N\).

The matrix A has m rows and N columns.

$$A = [\vec a_1 | \vec{a_2} | \vec{a_3} | ... | \vec{a_N}]$$


Suppose each \(\| \vec{a_j} \|_2 = 1\) for \(j = 1, 2, 3, ..., N\)

Let \(\mu\) be the coherence of A where

$$\mu = \underset{j \neq k}{max}| \langle a_j, a_k \rangle|$$

Show that

$$N^2 \leq m(M + (N^2 - N) \mu^2)$$

By rearranging terms, this can also be expressed as

$$\frac{N - m}{m(N - 1)} \leq \mu^2$$
\subsection{Hints}
\label{sec:org75e06b7}

Let \(H = AA^T\) and \(G = A^T A\).

Let \(tr(H)\) be the trace of H.

The following facts are useful:
\begin{enumerate}
\item \(tr(H) \leq \sqrt m \sqrt{tr(HH^T)}\)
\item \(tr(BB^T) = tr(B^T B)\)
\end{enumerate}

\section{Solution}
\label{sec:orgfe9f57f}

Let $$A^T A = \begin{bmatrix}
\langle \vec a_1, \vec a_1 \rangle & \langle \vec a_1, \vec a_2 \rangle & ... &
\langle \vec a_1, \vec a_N \rangle\\
\langle \vec a_2, \vec a_1 \rangle & \langle \vec a_2, \vec a_2 \rangle & ... &
\langle \vec a_2, \vec a_N \rangle\\
... & ... & ... & ... \\
\langle \vec a_N, \vec a_1 \rangle & ... & ... & \langle \vec a_N, \vec a_N \rangle
\end{bmatrix}
$$

\begin{equation}
\begin{split}
tr(A^T A) = tr(G) = \sum_{i = 1}^{N} \langle \vec a_i, \vec a_i \rangle = \sum_{i = 1}^{N} \|a_{ii} \|_2^2
\end{split}
\end{equation}

Let the dot product be represented as $$\langle \vec a, \vec a \rangle = \vec a^T a = \| a \|_2^2$$

Since \(\| a_{j} \| = 1\), then

\begin{equation}
\begin{split}
\sum_{i = 1}^{N} \| a_{ii} \|_2^2 = N
\end{split}
\end{equation}

Based on Hint (2), $$tr(AA^T) = tr(A^T A) = tr(H) = tr(G) = N$$


Let $$H^T = (AA^T)^T = A^T A = G$$ and $$G^T = (A^T A)^T = AA^T = H$$

Then \(tr(HH^T) = tr(G^T G)\)

Given that the trace is defined as the sum of the diagonal elements, then
\begin{equation}
\begin{split}
tr(G^T G) = \sum_{i = 1}^{N} \langle \vec a_i, \vec a_i \rangle
\end{split}
\end{equation}



Using (2) and the definitions for \(G^T, H^T\), Hint (1) can be rewritten as:

\begin{equation}
\begin{split}
tr(H) \leq & \sqrt m \sqrt{tr(HH^T)}\\
N \leq & \sqrt m \sqrt{tr(HH^T)}\\
N^2 \leq & m \ tr(HH^T)\\
N^2 \leq & m \ tr(G^T G)
\end{split}
\end{equation}

Since this is an inequality, substituting \(tr(G^T G)\) for a larger value means
that the inequality still holds. Consider the sum of dot products squared. It
can be said that \(tr(B) \leq \sum_{i, j}^{N} | \langle \vec b_i, \vec b_j
\rangle |^2\) for some square matrix B. Since the trace is the sum of diagonal
elements, this can be rewritten as

\begin{equation}
\begin{split}
tr(B) \leq tr(B) + \sum_{i \neq j}^{N} | \langle \vec b_i, \vec b_j \rangle|^2
\end{split}
\end{equation}

(4) can be further reduced using (5)

\begin{equation}
\begin{split}
N^2 \leq & m \ tr(G^T G)\\
N^2 \leq & m (tr(G) + \sum_{i \neq j}^{N} \langle \vec a_i, \vec a_j \rangle)\\
\frac{N^2}{m} \leq & N + \sum_{i \neq j}^{N} |\langle \vec a_i, \vec a_j \rangle|^2\\
\frac{N^2}{m} - N \leq & \sum_{i \neq j}^{N} | \langle \vec a_i, \vec a_j \rangle |^2\\
\to & \frac{N(N - m)}{m} \leq \sum_{i \neq j}^{N} | \langle \vec a_i, \vec a_j \rangle |^2
\end{split}
\end{equation}

By intuition, the average of a set of numbers is less than the maximum value in
that set.

\begin{equation}
\begin{split}
\frac{1}{N} \sum_{i = 1}^{N} a_i \leq {max} \ a_i
\end{split}
\end{equation}

Since \(\sum_{i \neq j}^{N} |\langle \vec a_i, \vec a_j \rangle |^2\) does not include the diagonal
elements, there are \(N(N - 1)\) elements. Thus we can rewrite (6) as

\begin{equation}
\begin{split}
\frac{N(N - m)}{m} \frac{1}{N(N - 1)} \sum_{i \neq j}^{N} | \langle \vec a_i, \vec a_j \rangle |^2 \leq \underset{i \neq j}{max} | \langle \vec a_i, \vec a_j \rangle |^2
\end{split}
\end{equation}

Since \(\sum_{i \neq j}^{N} |\langle \vec a_i, \vec a_j \rangle|^2\) can never be negative,
its presence in the inequality is not required and can be removed.

Thus

\begin{equation}
\begin{split}
\frac{N - m}{m(N - 1)} \leq \underset{i \neq j}{max} |\langle a_i, a_j \rangle|^2 = \mu^2
\end{split}
\end{equation}

[End]
\end{document}
